src/syntax.v
@@ -3,11 +3,21 @@
 Require Import ZArith.
 Require String.
 Require Import ListSet.
-Require Import comparable.
 Require set map.
 Require Import error.
+Require tez.
 
 (* source: http://doc.tzalpha.net/whitedoc/michelson.html#xii-full-grammar *)
+
+Inductive comparable_type : Set :=
+| string
+| nat
+| int
+| bytes
+| bool
+| mutez
+| key_hash
+| timestamp.
 
 Inductive type : Set :=
 | Comparable_type : comparable_type -> type
@@ -28,694 +38,267 @@ Inductive type : Set :=
 
 Coercion Comparable_type : comparable_type >-> type.
 
-Definition contract_env : Set := contract_constant -> type.
-
-Module neg.
-  Record class (a : comparable_type) :=
-    Class { neg : comparable_data a -> M Z }.
-
-  Structure type (a : comparable_type) := Pack { class_of : class a }.
-
-  Definition op (a : comparable_type) {e : type a} : comparable_data a -> M Z :=
-    neg _ (class_of a e).
-
-End neg.
-
-Canonical Structure neg_nat : neg.type nat :=
-  neg.Pack nat (neg.Class nat (fun x => Return _ (- Z.of_N x)%Z)).
-
-Canonical Structure neg_int : neg.type int :=
-  neg.Pack int (neg.Class int (fun x => Return _ (- x)%Z)).
-
-Module add.
-  Record class (a b c : comparable_type) :=
-    Class
-      { add : comparable_data a -> comparable_data b -> M (comparable_data c) }.
-
-  Structure type (a b : comparable_type) :=
-    Pack { ret : comparable_type; class_of : class a b ret }.
-
-  Definition op (a b : comparable_type) {e : type a b} :
-    comparable_data a -> comparable_data b ->
-    M (comparable_data (ret a b e)) :=
-    add _ _ _ (class_of a b e).
-
-End add.
-
-Canonical Structure add_nat_nat : add.type nat nat :=
-  add.Pack
-    nat nat nat
-    (add.Class nat nat nat (fun x y => Return _ (x + y)%N)).
-
-Canonical Structure add_nat_int : add.type nat int :=
-  add.Pack
-    nat int int
-    (add.Class nat int int (fun x y => Return _ (Z.of_N x + y)%Z)).
-
-Canonical Structure add_int_nat : add.type int nat :=
-  add.Pack
-    int nat int
-    (add.Class int nat int (fun x y => Return _ (x + Z.of_N y)%Z)).
-
-Canonical Structure add_int_int : add.type int int :=
-  add.Pack
-    int int int
-    (add.Class int int int (fun x y => Return _ (x + y)%Z)).
-
-Canonical Structure add_timestamp_int : add.type timestamp int :=
-  add.Pack
-    timestamp int timestamp
-    (add.Class timestamp int timestamp (fun x y => Return _ (x + y)%Z)).
-
-Canonical Structure add_int_timestamp : add.type int timestamp :=
-  add.Pack
-    int timestamp timestamp
-    (add.Class int timestamp timestamp (fun x y => Return _ (x + y)%Z)).
-
-Canonical Structure add_tez_tez : add.type mutez mutez :=
-  add.Pack
-    mutez mutez mutez
-    (add.Class
-       mutez mutez mutez
-       (fun x y =>
-          match tez.of_Z (tez.to_Z x + tez.to_Z y) with
-          | None => Failed _ Overflow
-          | Some t => Return _ t
-          end)).
-
-Module sub.
-  Record class (a b c : comparable_type) :=
-    Class
-      { sub : comparable_data a -> comparable_data b -> M (comparable_data c) }.
-
-  Structure type (a b : comparable_type) :=
-    Pack { ret : comparable_type; class_of : class a b ret }.
-
-  Definition op (a b : comparable_type) {e : type a b} :
-    comparable_data a -> comparable_data b ->
-    M (comparable_data (ret a b e)) :=
-    sub _ _ _ (class_of a b e).
-
-End sub.
-
-Canonical Structure sub_nat_nat : sub.type nat nat :=
-  sub.Pack _ _ _ (sub.Class nat nat int (fun x y => Return _ (Z.of_N x - Z.of_N y)%Z)).
-
-Canonical Structure sub_nat_int : sub.type nat int :=
-  sub.Pack _ _ _ (sub.Class nat int int (fun x y => Return _ (Z.of_N x - y)%Z)).
-
-Canonical Structure sub_int_nat : sub.type int nat :=
-  sub.Pack _ _ _ (sub.Class int nat int (fun x y => Return _ (x - Z.of_N y)%Z)).
-
-Canonical Structure sub_int_int : sub.type int int :=
-  sub.Pack _ _ _ (sub.Class int int int (fun x y => Return _ (x - y)%Z)).
-
-Canonical Structure sub_timestamp_int : sub.type timestamp int :=
-  sub.Pack _ _ _ (sub.Class timestamp int timestamp (fun x y => Return _ (x - y)%Z)).
-
-Canonical Structure sub_timestamp_timestamp : sub.type timestamp timestamp :=
-  sub.Pack _ _ _ (sub.Class timestamp timestamp int (fun x y => Return _ (x - y)%Z)).
-
-Canonical Structure sub_tez_tez : sub.type mutez mutez :=
-  sub.Pack
-    _ _ _ (sub.Class mutez mutez mutez
-    (fun x y =>
-       match tez.of_Z (tez.to_Z x - tez.to_Z y) with
-       | None => Failed _ Overflow
-       | Some t => Return _ t
-       end)).
-
-Module mul.
-  Record class (a b c : comparable_type) :=
-    Class
-      { mul : comparable_data a -> comparable_data b -> M (comparable_data c) }.
-
-  Structure type (a b : comparable_type) :=
-    Pack { ret : comparable_type; class_of : class a b ret }.
-
-  Definition op (a b : comparable_type) {e : type a b} :
-    comparable_data a -> comparable_data b ->
-    M (comparable_data (ret a b e)) :=
-    mul _ _ _ (class_of a b e).
-
-End mul.
-
-Canonical Structure mul_nat_nat : mul.type nat nat :=
-  mul.Pack _ _ _ (mul.Class nat nat nat (fun x y => Return _ (x * y)%N)).
-
-Canonical Structure mul_nat_int : mul.type nat int :=
-  mul.Pack _ _ _ (mul.Class nat int int (fun x y => Return _ (Z.of_N x * y)%Z)).
-
-Canonical Structure mul_int_nat : mul.type int nat :=
-  mul.Pack _ _ _ (mul.Class int nat int (fun x y => Return _ (x * Z.of_N y)%Z)).
-
-Canonical Structure mul_int_int : mul.type int int :=
-  mul.Pack _ _ _ (mul.Class int int int (fun x y => Return _ (x * y)%Z)).
-
-Canonical Structure mul_timestamp_int : mul.type timestamp int :=
-  mul.Pack _ _ _ (mul.Class timestamp int timestamp (fun x y => Return _ (x + y)%Z)).
-
-Canonical Structure mul_int_timestamp : mul.type int timestamp :=
-  mul.Pack _ _ _ (mul.Class int timestamp timestamp (fun x y => Return _ (x + y)%Z)).
-
-Canonical Structure mul_tez_nat : mul.type mutez nat :=
-  mul.Pack _ _ _ (mul.Class
-    mutez nat mutez
-    (fun x y =>
-       match tez.of_Z (tez.to_Z x * Z.of_N y) with
-       | None => Failed _ Overflow
-       | Some t => Return _ t
-       end)).
-
-Canonical Structure mul_nat_tez : mul.type nat mutez :=
-  mul.Pack _ _ _ (mul.Class
-    nat mutez mutez
-    (fun x y =>
-       match tez.of_Z (Z.of_N x * tez.to_Z y) with
-       | None => Failed _ Overflow
-       | Some t => Return _ t
-       end)).
-
-Module ediv.
-  Record class (a b c d : comparable_type) :=
-    Class
-      { ediv : comparable_data a -> comparable_data b ->
-               M (option (comparable_data c * comparable_data d)) }.
-
-  Structure type (a b : comparable_type) :=
-    Pack { quo : comparable_type; rem : comparable_type;
-           class_of : class a b quo rem }.
-
-  Definition op (a b : comparable_type) {e : type a b} :
-    comparable_data a -> comparable_data b ->
-    M (option (comparable_data (quo a b e) * comparable_data (rem a b e))) :=
-    ediv _ _ _ _ (class_of a b e).
-
-End ediv.
-
-Canonical Structure ediv_nat_nat : ediv.type nat nat :=
-  ediv.Pack _ _ _ _ (ediv.Class
-    nat nat nat nat
-    (fun x y =>
-       Return _
-               (if (y =? 0)%N then None
-                else Some ((x / y)%N, (x mod y)%N)))).
-
-Canonical Structure ediv_nat_int : ediv.type nat int :=
-  ediv.Pack _ _ _ _ (ediv.Class
-    nat int int nat
-    (fun x y =>
-       Return _
-               (if (y =? 0)%Z then None
-                else Some ((Z.of_N x / y)%Z, Z.to_N (Z.of_N x mod y)%Z)))).
-
-Canonical Structure ediv_int_nat : ediv.type int nat :=
-  ediv.Pack _ _ _ _ (ediv.Class
-    int nat int nat
-    (fun x y =>
-       Return _
-               (if (y =? 0)%N then None
-                else Some ((x / Z.of_N y)%Z, Z.to_N (x mod Z.of_N y)%Z)))).
-
-Canonical Structure ediv_int_int : ediv.type int int :=
-  ediv.Pack _ _ _ _ (ediv.Class
-    int int int nat
-    (fun x y =>
-       Return _
-               (if (y =? 0)%Z then None
-                else Some ((x / y)%Z, Z.to_N (x mod y)%Z)))).
-
-Canonical Structure ediv_tez_nat : ediv.type mutez nat :=
-  ediv.Pack _ _ _ _ (ediv.Class
-    mutez nat mutez mutez
-    (fun x y =>
-       Return _
-               (if (y =? 0)%N then None
-                else
-                  match tez.of_Z (tez.to_Z x / Z.of_N y)%Z,
-                        tez.of_Z (tez.to_Z x mod Z.of_N y)%Z
-                  with
-                  | Some quo, Some rem =>
-                    Some (quo, rem)
-                  | _, _ => None
-                              (* Should not happen but I am a bit lazy to prove it *)
-                  end))).
-
-Canonical Structure ediv_tez_tez : ediv.type mutez mutez :=
-  ediv.Pack _ _ _ _ (ediv.Class
-    mutez mutez nat mutez
-    (fun x y =>
-       Return _
-               (if (tez.to_Z y =? 0)%Z then None
-                else
-                  match Z.to_N (tez.to_Z x / tez.to_Z y)%Z,
-                        tez.of_Z (tez.to_Z x mod tez.to_Z y)%Z
-                  with
-                  | quo, Some rem =>
-                    Some (quo, rem)
-                  | _, _ => None
-                              (* Should not happen but I am a bit lazy to prove it *)
-                  end))).
-
-Module bitwise.
-  Record class (a : comparable_type) :=
-    Class
-      { bitwise_and : comparable_data a -> comparable_data a -> M (comparable_data a);
-        bitwise_or : comparable_data a -> comparable_data a -> M (comparable_data a);
-        bitwise_xor : comparable_data a -> comparable_data a -> M (comparable_data a) }.
-
-  Structure type (a : comparable_type) :=
-    Pack { class_of : class a }.
-
-  Definition and (a : comparable_type) {e : type a} :
-    comparable_data a -> comparable_data a ->
-    M (comparable_data a) :=
-    bitwise_and _ (class_of a e).
-
-  Definition or (a : comparable_type) {e : type a} :
-    comparable_data a -> comparable_data a ->
-    M (comparable_data a) :=
-    bitwise_or _ (class_of a e).
-
-  Definition xor (a : comparable_type) {e : type a} :
-    comparable_data a -> comparable_data a ->
-    M (comparable_data a) :=
-    bitwise_xor _ (class_of a e).
-
-End bitwise.
-
-Canonical Structure bitwise_bool : bitwise.type bool :=
-  bitwise.Pack _ (bitwise.Class
-    bool
-    (fun x y => Return _ (x && y)%bool)
-    (fun x y => Return _ (x || y)%bool)
-    (fun x y => Return _ (xorb x y))).
-
-Canonical Structure bitwise_nat : bitwise.type nat :=
-  bitwise.Pack _ (bitwise.Class
-    nat
-    (fun x y => Return _ (N.land x y))
-    (fun x y => Return _ (N.lor x y))
-    (fun x y => Return _ (N.lxor x y))).
-
-Module not.
-  Record class (a b : comparable_type) :=
-    Class
-      { bitwise_not : comparable_data a -> M (comparable_data b) }.
-
-  Structure type (a : comparable_type) :=
-    Pack { ret : comparable_type; class_of : class a ret }.
-
-  Definition not (a : comparable_type) {e : type a} :
-    comparable_data a ->
-    M (comparable_data (ret a e)) :=
-    bitwise_not _ _ (class_of a e).
-
-End not.
-
-Canonical Structure bitwise_not_bool : not.type bool :=
-  not.Pack _ _ (not.Class bool bool (fun x => Return _ (negb x))).
-
-Canonical Structure bitwise_not_int : not.type int :=
-  not.Pack _ _ (not.Class
-    int int
-    (fun x => Return _ (- 1 - x)%Z)).
-
-Canonical Structure bitwise_not_nat : not.type nat :=
-  not.Pack _ _ (not.Class
-    nat int
-    (fun x => Return _ (- 1 - Z.of_N x)%Z)).
-
-Module mem.
-  Definition top_type := type.
-
-  Record class (data : type -> Set) (key : comparable_type) (collection : type) : Set :=
-    Class
-      { mem : comparable_data key -> data collection ->
-              M Datatypes.bool }.
-
-  Structure type (data : type -> Set) (key : comparable_type) :=
-    Pack { collection : top_type;
-           class_of : class data key collection }.
-
-  Definition op data key e := mem _ _ _ (class_of data key e).
-End mem.
-
-Module update.
-  Definition top_type := type.
-
-  Record class (data : type -> Set) (key : comparable_type) (collection : type)
-               (opt_val : type) : Set :=
-    Class
-      { update : comparable_data key ->
-                 data opt_val ->
-                 data collection ->
-                 M (data collection) }.
-  Structure type (data : type -> Set) (key : comparable_type) :=
-    Pack { collection : top_type;
-           opt_val : top_type;
-           class_of : class data key collection opt_val }.
-
-  Definition op data key e := update _ _ _ _ (class_of data key e).
-End update.
-
-Module reduce.
-  Definition top_type := type.
-
-  Record class (data : type -> Set) (collection : type)
-         (entry : type) : Set :=
-    Class
-      { reduce : forall b : type,
-          ((data entry * data b) -> M (data b)) ->
-          data collection -> data b -> M (data b) }.
-  Structure type (data : type -> Set) :=
-    Pack { collection : top_type;
-           entry : top_type;
-           class_of : class data collection entry }.
-
-  Definition op data e := reduce _ _ _ (class_of data e).
-End reduce.
-
-Module size.
-  Definition top_type := type.
-
-  Record class (data : type -> Set) (collection : type) : Set :=
-    Class
-      { size : data collection -> M N }.
-
-  Structure type (data : type -> Set) :=
-    Pack { collection : top_type;
-           class_of : class data collection }.
-
-  Definition op data e := size _ _ (class_of data e).
-End size.
-
-Module get.
-  Definition top_type := type.
-
-  Record class (data : type -> Set) (collection : type) (key : comparable_type) (val : type) : Set :=
-    Class
-      { get : comparable_data key -> data collection -> M (data (option_ val)) }.
-
-  Structure type (data : type -> Set) (key : comparable_type) :=
-    Pack { collection : top_type;
-           val : top_type;
-           class_of : class data collection key val }.
-
-  Definition op data key e := get _ _ _ _ (class_of data key e).
-End get.
-
-Module MAP.
-  Definition top_type := type.
-
-  Record class (data : type -> Set) (collection : type -> type)
-         (val : type) (entry : type) : Set :=
-    Class
-      { map : forall b, (data entry -> M (data b)) ->
-                        data (collection val) ->
-                        M (data (collection b)) }.
-
-  Structure type (data : type -> Set) :=
-    Pack { collection : top_type -> top_type;
-           val : top_type;
-           entry : top_type;
-           class_of : class data collection val entry }.
-
-  Definition op data e := map _ _ _ _ (class_of data e).
-
-End MAP.
-
-Module string_like.
-  Record class (a : comparable_type) :=
-    Class
-      { slice_ : comparable_data nat -> comparable_data nat ->
-                 comparable_data a -> M (option (comparable_data string));
-        concat_ : comparable_data a -> comparable_data a -> M (comparable_data a)}.
-
-  Structure type (a : comparable_type) :=
-    Pack { class_of : class a }.
-
-  Definition slice (a : comparable_type) {e : type a} :
-    comparable_data nat ->
-    comparable_data nat ->
-    comparable_data a ->
-    M (option (comparable_data string)) :=
-    slice_ _ (class_of a e).
-
-  Definition concat (a : comparable_type) {e : type a} :
-    comparable_data a ->
-    comparable_data a ->
-    M (comparable_data a) :=
-    concat_ _ (class_of a e).
-
-End string_like.
-
-Definition str_slice (n1 n2 : N.t) (s : str) : M (option str) :=
-  if (n1 + n2 <=? N.of_nat (String.length s))%N then
-    Return _ (Some (String.substring (N.to_nat n1) (N.to_nat n2) s))
-  else Return _ None.
-
-Canonical Structure string_like_string : string_like.type string :=
-  string_like.Pack _
-    (string_like.Class string str_slice (fun s1 s2 => Return _ (String.append s1 s2))).
-
-Canonical Structure string_like_bytes : string_like.type bytes :=
-  string_like.Pack _
-    (string_like.Class bytes str_slice (fun s1 s2 => Return _ (String.append s1 s2))).
-
 Infix ":::" := (@cons type) (at level 60, right associativity).
+
+
+Section Overloading.
+
+(* Boolean binary opertations (OR, XOR, AND) are overloaded as bitwise operations for nat. *)
+Inductive bitwise_variant : type -> Set :=
+| Bitwise_variant_bool : bitwise_variant bool
+| Bitwise_variant_nat : bitwise_variant nat.
+Structure bitwise_struct (a : type) :=
+  Mk_bitwise { bitwise_variant_field : bitwise_variant a }.
+Canonical Structure bitwise_bool : bitwise_struct bool := {| bitwise_variant_field := Bitwise_variant_bool |}.
+Canonical Structure bitwise_nat : bitwise_struct nat := {| bitwise_variant_field := Bitwise_variant_nat |}.
+
+(* Logical negation is also overloaded for int *)
+Inductive not_variant : type -> type -> Set :=
+| Not_variant_bool : not_variant bool bool
+| Not_variant_nat : not_variant nat int
+| Not_variant_int : not_variant int int.
+Structure not_struct (a : type) :=
+  Mk_not { not_ret_type : type; not_variant_field : not_variant a not_ret_type }.
+Canonical Structure not_bool : not_struct bool :=
+  {| not_variant_field := Not_variant_bool |}.
+Canonical Structure not_nat : not_struct nat :=
+  {| not_variant_field := Not_variant_nat |}.
+Canonical Structure not_int : not_struct int :=
+  {| not_variant_field := Not_variant_int |}.
+
+(* NEG takes either a nat or an int as argument *)
+Inductive neg_variant : type -> Set :=
+| Neg_variant_nat : neg_variant nat
+| Neg_variant_int : neg_variant int.
+Structure neg_struct (a : type) := Mk_neg { neg_variant_field : neg_variant a }.
+Canonical Structure neg_nat : neg_struct nat :=
+  {| neg_variant_field := Neg_variant_nat |}.
+Canonical Structure neg_int : neg_struct int :=
+  {| neg_variant_field := Neg_variant_int |}.
+
+(* ADD *)
+Inductive add_variant : type -> type -> type -> Set :=
+| Add_variant_nat_nat : add_variant nat nat nat
+| Add_variant_nat_int : add_variant nat int int
+| Add_variant_int_nat : add_variant int nat int
+| Add_variant_int_int : add_variant int int int
+| Add_variant_timestamp_int : add_variant timestamp int timestamp
+| Add_variant_int_timestamp : add_variant int timestamp timestamp
+| Add_variant_tez_tez : add_variant mutez mutez mutez.
+Structure add_struct (a b : type) :=
+  Mk_add { add_ret_type : type; add_variant_field : add_variant a b add_ret_type }.
+Canonical Structure add_nat_nat : add_struct nat nat :=
+  {| add_variant_field := Add_variant_nat_nat |}.
+Canonical Structure add_nat_int : add_struct nat int :=
+  {| add_variant_field := Add_variant_nat_int |}.
+Canonical Structure add_int_nat : add_struct int nat :=
+  {| add_variant_field := Add_variant_int_nat |}.
+Canonical Structure add_int_int : add_struct int int :=
+  {| add_variant_field := Add_variant_int_int |}.
+Canonical Structure add_timestamp_int : add_struct timestamp int :=
+  {| add_variant_field := Add_variant_timestamp_int |}.
+Canonical Structure add_int_timestamp : add_struct int timestamp :=
+  {| add_variant_field := Add_variant_int_timestamp |}.
+Canonical Structure add_tez_tez : add_struct mutez mutez :=
+  {| add_variant_field := Add_variant_tez_tez |}.
+
+(* SUB *)
+Inductive sub_variant : type -> type -> type -> Set :=
+| Sub_variant_nat_nat : sub_variant nat nat int
+| Sub_variant_nat_int : sub_variant nat int int
+| Sub_variant_int_nat : sub_variant int nat int
+| Sub_variant_int_int : sub_variant int int int
+| Sub_variant_timestamp_int : sub_variant timestamp int timestamp
+| Sub_variant_timestamp_timestamp : sub_variant timestamp timestamp int
+| Sub_variant_tez_tez : sub_variant mutez mutez mutez.
+Structure sub_struct (a b : type) :=
+  Mk_sub { sub_ret_type : type; sub_variant_field : sub_variant a b sub_ret_type }.
+Canonical Structure sub_nat_nat : sub_struct nat nat :=
+  {| sub_variant_field := Sub_variant_nat_nat |}.
+Canonical Structure sub_nat_int : sub_struct nat int :=
+  {| sub_variant_field := Sub_variant_nat_int |}.
+Canonical Structure sub_int_nat : sub_struct int nat :=
+  {| sub_variant_field := Sub_variant_int_nat |}.
+Canonical Structure sub_int_int : sub_struct int int :=
+  {| sub_variant_field := Sub_variant_int_int |}.
+Canonical Structure sub_timestamp_int : sub_struct timestamp int :=
+  {| sub_variant_field := Sub_variant_timestamp_int |}.
+Canonical Structure sub_timestamp_timestamp : sub_struct timestamp timestamp :=
+  {| sub_variant_field := Sub_variant_timestamp_timestamp |}.
+Canonical Structure sub_tez_tez : sub_struct mutez mutez :=
+  {| sub_variant_field := Sub_variant_tez_tez |}.
+
+(* MUL *)
+Inductive mul_variant : type -> type -> type -> Set :=
+| Mul_variant_nat_nat : mul_variant nat nat nat
+| Mul_variant_nat_int : mul_variant nat int int
+| Mul_variant_int_nat : mul_variant int nat int
+| Mul_variant_int_int : mul_variant int int int
+| Mul_variant_tez_nat : mul_variant mutez nat mutez
+| Mul_variant_nat_tez : mul_variant nat mutez mutez.
+Structure mul_struct (a b : type) :=
+  Mk_mul { mul_ret_type : type; mul_variant_field : mul_variant a b mul_ret_type }.
+Canonical Structure mul_nat_nat : mul_struct nat nat :=
+  {| mul_variant_field := Mul_variant_nat_nat |}.
+Canonical Structure mul_nat_int : mul_struct nat int :=
+  {| mul_variant_field := Mul_variant_nat_int |}.
+Canonical Structure mul_int_nat : mul_struct int nat :=
+  {| mul_variant_field := Mul_variant_int_nat |}.
+Canonical Structure mul_int_int : mul_struct int int :=
+  {| mul_variant_field := Mul_variant_int_int |}.
+Canonical Structure mul_tez_nat : mul_struct mutez nat :=
+  {| mul_variant_field := Mul_variant_tez_nat |}.
+Canonical Structure mul_nat_tez : mul_struct nat mutez :=
+  {| mul_variant_field := Mul_variant_nat_tez |}.
+
+(* EDIV *)
+Inductive ediv_variant : type -> type -> type -> type -> Set :=
+| Ediv_variant_nat_nat : ediv_variant nat nat nat nat
+| Ediv_variant_nat_int : ediv_variant nat int int nat
+| Ediv_variant_int_nat : ediv_variant int nat int nat
+| Ediv_variant_int_int : ediv_variant int int int nat
+| Ediv_variant_tez_nat : ediv_variant mutez nat mutez mutez
+| Ediv_variant_tez_tez : ediv_variant mutez mutez nat mutez.
+Structure ediv_struct (a b : type) :=
+  Mk_ediv { ediv_quo_type : type; ediv_rem_type : type;
+            ediv_variant_field : ediv_variant a b ediv_quo_type ediv_rem_type }.
+Canonical Structure ediv_nat_nat : ediv_struct nat nat :=
+  {| ediv_variant_field := Ediv_variant_nat_nat |}.
+Canonical Structure ediv_nat_int : ediv_struct nat int :=
+  {| ediv_variant_field := Ediv_variant_nat_int |}.
+Canonical Structure ediv_int_nat : ediv_struct int nat :=
+  {| ediv_variant_field := Ediv_variant_int_nat |}.
+Canonical Structure ediv_int_int : ediv_struct int int :=
+  {| ediv_variant_field := Ediv_variant_int_int |}.
+Canonical Structure ediv_tez_nat : ediv_struct mutez nat :=
+  {| ediv_variant_field := Ediv_variant_tez_nat |}.
+Canonical Structure ediv_tez_tez : ediv_struct mutez mutez :=
+  {| ediv_variant_field := Ediv_variant_tez_tez |}.
+
+(* SLICE and CONCAT *)
+Inductive stringlike_variant : type -> Set :=
+| Stringlike_variant_string : stringlike_variant string
+| Stringlike_variant_bytes : stringlike_variant bytes.
+Structure stringlike_struct (a : type) :=
+  Mk_stringlike { stringlike_variant_field : stringlike_variant a }.
+Canonical Structure stringlike_string : stringlike_struct string :=
+  {| stringlike_variant_field := Stringlike_variant_string |}.
+Canonical Structure stringlike_bytes : stringlike_struct bytes :=
+  {| stringlike_variant_field := Stringlike_variant_bytes |}.
+
+(* SIZE *)
+Inductive size_variant : type -> Set :=
+| Size_variant_set a : size_variant (set_ a)
+| Size_variant_map key val : size_variant (map key val)
+| Size_variant_list a : size_variant (list_ a)
+| Size_variant_string : size_variant string
+| Size_variant_bytes : size_variant bytes.
+Structure size_struct (a : type) :=
+  Mk_size { size_variant_field : size_variant a }.
+Canonical Structure size_set a : size_struct (set_ a) :=
+  {| size_variant_field := Size_variant_set a |}.
+Canonical Structure size_map key val : size_struct (map key val) :=
+  {| size_variant_field := Size_variant_map key val |}.
+Canonical Structure size_list a : size_struct (list_ a) :=
+  {| size_variant_field := Size_variant_list a |}.
+Canonical Structure size_string : size_struct string :=
+  {| size_variant_field := Size_variant_string |}.
+Canonical Structure size_bytes : size_struct bytes :=
+  {| size_variant_field := Size_variant_bytes |}.
+
+(* MEM *)
+Inductive mem_variant : comparable_type -> type -> Set :=
+| Mem_variant_set a : mem_variant a (set_ a)
+| Mem_variant_map key val : mem_variant key (map key val)
+| Mem_variant_bigmap key val : mem_variant key (big_map key val).
+Structure mem_struct (key : comparable_type) (a : type) :=
+  Mk_mem { mem_variant_field : mem_variant key a }.
+Canonical Structure mem_set a : mem_struct a (set_ a) :=
+  {| mem_variant_field := Mem_variant_set a |}.
+Canonical Structure mem_map key val : mem_struct key (map key val) :=
+  {| mem_variant_field := Mem_variant_map key val |}.
+Canonical Structure mem_bigmap key val : mem_struct key (big_map key val) :=
+  {| mem_variant_field := Mem_variant_bigmap key val |}.
+
+(* UPDATE *)
+Inductive update_variant : comparable_type -> type -> type -> Set :=
+| Update_variant_set a : update_variant a bool (set_ a)
+| Update_variant_map key val : update_variant key (option_ val) (map key val)
+| Update_variant_bigmap key val : update_variant key (option_ val) (big_map key val).
+Structure update_struct key val collection :=
+  Mk_update { update_variant_field : update_variant key val collection }.
+Canonical Structure update_set a : update_struct a bool (set_ a) :=
+  {| update_variant_field := Update_variant_set a |}.
+Canonical Structure update_mao key val :=
+  {| update_variant_field := Update_variant_map key val |}.
+Canonical Structure update_bigmap key val :=
+  {| update_variant_field := Update_variant_bigmap key val |}.
+
+(* ITER *)
+Inductive iter_variant : type -> type -> Set :=
+| Iter_variant_set (a : comparable_type) : iter_variant a (set_ a)
+| Iter_variant_map (key : comparable_type) val : iter_variant (pair key val) (map key val)
+| Iter_variant_list a : iter_variant a (list_ a).
+Structure iter_struct collection :=
+  Mk_iter { iter_elt_type : type;
+            iter_variant_field : iter_variant iter_elt_type collection }.
+Canonical Structure iter_set a : iter_struct (set_ a) :=
+  {| iter_variant_field := Iter_variant_set a |}.
+Canonical Structure iter_map key val : iter_struct (map key val) :=
+  {| iter_variant_field := Iter_variant_map key val |}.
+Canonical Structure iter_list a : iter_struct (list_ a) :=
+  {| iter_variant_field := Iter_variant_list a |}.
+
+(* GET *)
+Inductive get_variant : comparable_type -> type -> type -> Set :=
+| Get_variant_map key val : get_variant key val (map key val)
+| Get_variant_bigmap key val : get_variant key val (big_map key val).
+Structure get_struct key collection :=
+  Mk_get { get_val_type : type;
+           get_variant_field : get_variant key get_val_type collection }.
+Canonical Structure get_map key val : get_struct key (map key val) :=
+  {| get_variant_field := Get_variant_map key val |}.
+Canonical Structure get_bigmap key val : get_struct key (big_map key val) :=
+  {| get_variant_field := Get_variant_bigmap key val |}.
+
+(* MAP *)
+Inductive map_variant : type -> type -> type -> type -> Set :=
+| Map_variant_map (key : comparable_type) val b :
+    map_variant (pair key val) b (map key val) (map key b)
+| Map_variant_list a b :
+    map_variant a b (list_ a) (list_ b).
+Structure map_struct collection b :=
+  Mk_map { map_in_type : type; map_out_collection_type : type;
+           map_variant_field :
+             map_variant map_in_type b collection map_out_collection_type }.
+Canonical Structure map_map key val b : map_struct (map key val) b :=
+  {| map_variant_field := Map_variant_map key val b |}.
+Canonical Structure map_list a b : map_struct (list_ a) b :=
+  {| map_variant_field := Map_variant_list a b |}.
+
+End Overloading.
+
+Definition str := String.string.
+Inductive timestamp_constant : Set := Mk_timestamp : str -> timestamp_constant.
+Inductive signature_constant : Set := Mk_sig : str -> signature_constant.
+Inductive key_constant : Set := Mk_key : str -> key_constant.
+Inductive key_hash_constant : Set := Mk_key_hash : str -> key_hash_constant.
+Inductive tez_constant : Set := Mk_tez : str -> tez_constant.
+Inductive contract_constant : Set := Mk_contract : str -> contract_constant.
+Inductive address_constant : Set := Mk_address : str -> address_constant.
+Inductive operation_constant : Set := Mk_operation : str -> operation_constant.
+Inductive mutez_constant : Set := Mk_mutez : tez.mutez -> mutez_constant.
 
 Section syntax.
 
-Parameter e : contract_env.
-Parameter ae : address_constant -> type.
+Context {get_contract_type : contract_constant -> M type}.
 
-Fixpoint data (a : type) {struct a} : Set :=
-  match a with
-  | Comparable_type b => comparable_data b
-  | address => address_constant
-  | signature => signature_constant
-  | operation => operation_constant
-  | key => key_constant
-  | unit => Datatypes.unit
-  | pair a b => data a * data b
-  | or a b => sum (data a) (data b)
-  | option_ a => option (data a)
-  | list_ a => list (data a)
-  | set_ a => set.set (comparable_data a) (compare a)
-  | map a b => map.map (comparable_data a) (data b) (compare a)
-  | big_map a b => map.map (comparable_data a) (data b) (compare a)
-  | lambda a b => data a -> M (data b)
-  | contract a => {s : contract_constant | e s = a }
-  end.
 
-Record node : Set :=
-  mk_node
-    {
-      create_contract : forall g p,
-          comparable_data key_hash ->
-          option (comparable_data key_hash) ->
-          Datatypes.bool -> Datatypes.bool -> tez.mutez ->
-          (data (pair p g) -> M (data (pair (list_ operation) g))) ->
-          data g -> M (data (pair operation address));
-      create_account :
-          comparable_data key_hash ->
-          option (comparable_data key_hash) ->
-          Datatypes.bool -> tez.mutez ->
-          M (data operation * data (contract unit));
-      transfer_tokens : forall p,
-          data p -> tez.mutez -> data (contract p) ->
-          M (data operation);
-      set_delegate : option (comparable_data key_hash) ->
-                     M (data operation);
-      balance : M tez.mutez;
-      address_ : forall p, data (contract p) -> M (data address);
-      contract_ : forall p, data address -> M (option (data (contract p)));
-      source : M (data address);
-      sender : M (data address);
-      self : forall p, M (data (contract p));
-      amount : M tez.mutez;
-      implicit_account :
-        comparable_data key_hash -> M (data (contract unit));
-      steps_to_quota : M N;
-      now : M (comparable_data timestamp);
-      hash_key : data key -> M (comparable_data key_hash);
-      pack : forall a, data a -> M str;
-      unpack : forall a, str -> M (option (data a));
-      blake2b : str -> M str;
-      sha256 : str -> M str;
-      sha512 : str -> M str;
-      check_signature :
-        data key -> data signature -> String.string -> M Datatypes.bool
-    }.
-
-Canonical Structure mem_set (key : comparable_type) :=
-  {| mem.collection := set_ key;
-     mem.class_of :=
-       {| mem.mem := fun k (s : data (set_ key)) =>
-                       Return _ (set.mem _ _ (compare_eq_iff key) k s) |} |}.
-
-Canonical Structure update_set (key : comparable_type) :=
-  {| update.collection := set_ key;
-     update.opt_val := bool;
-     update.class_of :=
-       {| update.update := fun k (v : data bool) (s : data (set_ key)) =>
-                             Return _
-                                     (set.update _ _
-                                                 (compare_eq_iff key)
-                                                 (lt_trans key)
-                                                 (gt_trans key) k s v) |} |}.
-
-Canonical Structure mem_map (key : comparable_type) (val : type) :=
-  {| mem.collection := map key val;
-     mem.class_of :=
-       {| mem.mem := fun k (s : data (map key val)) =>
-                       Return _ (map.mem _ _ _ k s) |} |}.
-
-Canonical Structure update_map (key : comparable_type) (val : type) :=
-  {| update.collection := map key val;
-     update.opt_val := option_ val;
-     update.class_of :=
-       {| update.update := fun k
-                               (v : data (option_ val)) (s : data (map key val)) =>
-                             Return _
-                                     (map.update _ _ _
-                                                 (comparable.compare_eq_iff key)
-                                                 (comparable.lt_trans key)
-                                                 (comparable.gt_trans key) k v s)
-       |} |}.
-
-Canonical Structure mem_big_map (key : comparable_type) (val : type) :=
-  {| mem.collection := big_map key val;
-     mem.class_of :=
-       {| mem.mem := fun k (s : data (big_map key val)) =>
-                       Return _ (map.mem _ _ _ k s) |} |}.
-
-Canonical Structure update_big_map (key : comparable_type) (val : type) :=
-  {| update.collection := big_map key val;
-     update.opt_val := option_ val;
-     update.class_of :=
-       {| update.update := fun k (v : data (option_ val)) (s : data (big_map key val)) =>
-                             Return _
-                                     (map.update _ _ _
-                                                 (comparable.compare_eq_iff key)
-                                                 (comparable.lt_trans key)
-                                                 (comparable.gt_trans key) k v s)
-       |} |}.
-
-Canonical Structure reduce_set (key : comparable_type) :=
-  {| reduce.collection := set_ key;
-     reduce.entry := key;
-     reduce.class_of :=
-       reduce.Class
-         data (set_ key) key
-         (fun (B : type) (f : (data key * data B) -> M (data B))
-              (s : data (set_ key)) (b : data B) =>
-            set.reduce
-              (comparable_data key)
-              (comparable.compare key)
-              (data B) f b s) |}.
-
-Canonical Structure reduce_map (key : comparable_type) (val : type) :=
-  {| reduce.collection := map key val;
-     reduce.entry := pair key val;
-     reduce.class_of :=
-       reduce.Class
-         data (map key val) (pair key val)
-         (fun (B : type) (f : (data (pair key val) * data B) -> M (data B))
-              (s : data (map key val)) (b : data B) =>
-            set.reduce
-              (data key * data val)
-              (map.map_compare (comparable_data key) (data val) _)
-              (data B) f b s) |}.
-
-Canonical Structure reduce_list (a : type) :=
-  {| reduce.collection := list_ a;
-     reduce.entry := a;
-     reduce.class_of :=
-       reduce.Class
-         data (list_ a) a
-         (fun (B : type) (f : (data a * data B) -> M (data B))
-              (s : data (list_ a)) (b : data B) =>
-            set.list_reduce
-              (data a)
-              (data B) f b s) |}.
-
-Canonical Structure size_set (key : comparable_type) :=
-  {| size.collection := set_ key;
-     size.class_of :=
-       {| size.size := fun (s : data (set_ key)) =>
-                         let (l, _) := s in
-                         Return _ (N.of_nat (List.length l)) |}
-       |}.
-
-Canonical Structure size_map (key : comparable_type) (val : type) :=
-  {| size.collection := map key val;
-     size.class_of :=
-       {| size.size := fun (s : data (map key val)) =>
-                         let (l, _) := s in
-                         Return _ (N.of_nat (List.length l)) |}
-       |}.
-
-Canonical Structure size_list (a : type) :=
-  {| size.collection := list_ a;
-     size.class_of :=
-       {| size.size := fun (l : data (list_ a)) =>
-                         Return _ (N.of_nat (List.length l)) |}
-       |}.
-
-Canonical Structure size_string :=
-  {| size.collection := string;
-     size.class_of :=
-       {| size.size := fun (s : data string) =>
-                         Return _ (N.of_nat (String.length s)) |}
-       |}.
-
-Canonical Structure size_bytes :=
-  {| size.collection := bytes;
-     size.class_of :=
-       {| size.size := fun (s : data bytes) =>
-                         Return _ (N.of_nat (String.length s)) |}
-       |}.
-
-Canonical Structure get_map (key : comparable_type) (val : type) :=
-  {| get.collection := map key val;
-     get.class_of :=
-       {| get.get := fun k (s : data (map key val)) =>
-                       Return _ (map.get _ _ _ k s) |}
-       |}.
-
-Canonical Structure get_big_map (key : comparable_type) (val : type) :=
-  {| get.collection := big_map key val;
-     get.class_of :=
-       {| get.get := fun k (s : data (big_map key val)) =>
-                       Return _ (map.get _ _ _ k s) |}
-       |}.
-
-Canonical Structure map_map (key : comparable_type) (val : type) :=
-  {| MAP.collection := map key;
-     MAP.entry := pair key val;
-     MAP.class_of :=
-       MAP.Class
-         data
-         (map key)
-         val
-         (pair key val)
-         (fun B f m => map.map_fun _ _ _ _ f m) |}.
-
-Canonical Structure map_list (a : type) :=
-  {| MAP.collection := list_;
-     MAP.entry := a;
-     MAP.class_of :=
-       MAP.Class
-         data
-         list_
-         a
-         a
-         (fun B f l => map.list_map _ _ f l) |}.
+Inductive elt_pair (a b : Set) : Set :=
+| Elt : a -> b -> elt_pair a b.
 
 Inductive instruction : list type -> list type -> Set :=
-| NOOP {A} : instruction A A
+| NOOP {A} : instruction A A    (* Undocumented *)
 | FAILWITH {A B a} : instruction (a ::: A) B
 | SEQ {A B C} : instruction A B -> instruction B C -> instruction A C
 (* The instruction SEQ I C is written "{ I ; C }" in Michelson *)
@@ -731,7 +314,7 @@ this constructor "IF" but we can make a notation for it. *)
 | DROP {a A} : instruction (a :: A) A
 | DUP {a A} : instruction (a ::: A) (a ::: a ::: A)
 | SWAP {a b A} : instruction (a ::: b ::: A) (b ::: a ::: A)
-| PUSH (a : type) (x : data a) {A} : instruction A (a :: A)
+| PUSH (a : type) (x : concrete_data a) {A} : instruction A (a :: A)
 | UNIT {A} : instruction A (unit :: A)
 | LAMBDA (a b : type) {A} : instruction (a :: nil) (b :: nil) ->
                      instruction A (lambda a b :: A)
@@ -741,47 +324,44 @@ this constructor "IF" but we can make a notation for it. *)
 | GT {S} : instruction (int ::: S) (bool ::: S)
 | LE {S} : instruction (int ::: S) (bool ::: S)
 | GE {S} : instruction (int ::: S) (bool ::: S)
-| OR {b} {s : bitwise.type b} {S} : instruction (b ::: b ::: S) (b ::: S)
-| AND {b} {s : bitwise.type b} {S} : instruction (b ::: b ::: S) (b ::: S)
-| XOR {b} {s : bitwise.type b} {S} : instruction (b ::: b ::: S) (b ::: S)
-| NOT {b} {s : not.type b} {S} : instruction (b ::: S) (not.ret _ s ::: S)
-| NEG {n} {s : neg.type n} {S} : instruction (n ::: S) (int ::: S)
+| OR {b} {s : bitwise_struct b} {S} : instruction (b ::: b ::: S) (b ::: S)
+| AND {b} {s : bitwise_struct b} {S} : instruction (b ::: b ::: S) (b ::: S)
+| XOR {b} {s : bitwise_struct b} {S} : instruction (b ::: b ::: S) (b ::: S)
+| NOT {b} {s : not_struct b} {S} : instruction (b ::: S) (not_ret_type _ s ::: S)
+| NEG {n} {s : neg_struct n} {S} : instruction (n ::: S) (int ::: S)
 | ABS {S} : instruction (int ::: S) (nat ::: S)
-| ADD {a b} {s : add.type a b} {S} :
-    instruction (a ::: b ::: S) (add.ret _ _ s ::: S)
-| SUB {a b} {s : sub.type a b} {S} :
-    instruction (a ::: b ::: S) (sub.ret _ _ s ::: S)
-| MUL {a b} {s : mul.type a b} {S} :
-    instruction (a ::: b ::: S) (mul.ret _ _ s ::: S)
-| EDIV {a b} {s : ediv.type a b} {S} : instruction (a ::: b ::: S) (option_ (pair (ediv.quo _ _ s) (ediv.rem _ _ s)) :: S)
+| ADD {a b} {s : add_struct a b} {S} :
+    instruction (a ::: b ::: S) (add_ret_type _ _ s ::: S)
+| SUB {a b} {s : sub_struct a b} {S} :
+    instruction (a ::: b ::: S) (sub_ret_type _ _ s ::: S)
+| MUL {a b} {s : mul_struct a b} {S} :
+    instruction (a ::: b ::: S) (mul_ret_type _ _ s ::: S)
+| EDIV {a b} {s : ediv_struct a b} {S} : instruction (a ::: b ::: S) (option_ (pair (ediv_quo_type _ _ s) (ediv_rem_type _ _ s)) :: S)
 | LSL {S} : instruction (nat ::: nat ::: S) (nat ::: S)
 | LSR {S} : instruction (nat ::: nat ::: S) (nat ::: S)
 | COMPARE {a : comparable_type} {S} : instruction (a ::: a ::: S) (int ::: S)
-| CONCAT {S a} {i : string_like.type a} : instruction (a ::: a ::: S) (a ::: S)
-| SIZE {i : size.type data} {S} :
-    instruction (size.collection _ i ::: S) (nat ::: S)
-| SLICE {S a} {i : string_like.type a} :
-    instruction (nat ::: nat ::: a ::: S) (option_ string ::: S)
+| CONCAT {a} {i : stringlike_struct a} {S} : instruction (a ::: a ::: S) (a ::: S)
+| SIZE {a} {i : size_struct a} {S} :
+    instruction (a ::: S) (nat ::: S)
+| SLICE {a} {i : stringlike_struct a} {S} :
+    instruction (nat ::: nat ::: a ::: S) (option_ a ::: S)
 | PAIR {a b S} : instruction (a ::: b ::: S) (pair a b :: S)
 | CAR {a b S} : instruction (pair a b :: S) (a :: S)
 | CDR {a b S} : instruction (pair a b :: S) (b :: S)
-| EMPTY_SET (elt : comparable_type) {S} : instruction S (set_ elt ::: S)
-| MEM {elt : comparable_type} {i : mem.type data elt} {S} :
-    instruction (elt ::: mem.collection _ _ i ::: S) (bool ::: S)
-| UPDATE {elt : comparable_type} {i : update.type data elt} {S} :
-    instruction (elt ::: update.opt_val _ _ i ::: update.collection _ _ i ::: S) (update.collection _ _ i ::: S)
-| ITER_set {elt : comparable_type} {A} :
-    instruction (elt ::: A) A -> instruction (set_ elt :: A) A
+| EMPTY_SET elt {S} : instruction S (set_ elt ::: S)
+| MEM {elt a} {i : mem_struct elt a} {S} :
+    instruction (elt ::: a ::: S) (bool ::: S)
+| UPDATE {elt val collection} {i : update_struct elt val collection} {S} :
+    instruction (elt ::: val ::: collection ::: S) (collection ::: S)
+| ITER {collection} {i : iter_struct collection} {A} :
+    instruction (iter_elt_type _ i ::: A) A -> instruction (collection :: A) A
 | EMPTY_MAP (key : comparable_type) (val : type) {S} :
     instruction S (map key val :: S)
-| GET {key : comparable_type} {i : get.type data key} {S} :
-    instruction (key ::: get.collection _ _ i ::: S) (option_ (get.val _ _ i) :: S)
-| MAP_map_body {key : comparable_type} {val b A} :
-    instruction (pair key val :: A) (b :: A) ->
-    instruction (map key val :: A) (map key b :: A)
-| ITER_map {elt : comparable_type} {val A} :
-    instruction (pair elt val :: A) A ->
-    instruction (map elt val :: A) A
+| GET {key collection} {i : get_struct key collection} {S} :
+    instruction (key ::: collection ::: S) (option_ (get_val_type _ _ i) :: S)
+| MAP {collection b} {i : map_struct collection b} {A} :
+    instruction (map_in_type _ _ i :: A) (b :: A) ->
+    instruction (collection :: A) (map_out_collection_type _ _ i :: A)
 | SOME {a S} : instruction (a :: S) (option_ a :: S)
 | NONE (a : type) {S} : instruction S (option_ a :: S)
 (* Not the one documented, see https://gitlab.com/tezos/tezos/issues/471 *)
@@ -804,10 +384,6 @@ this constructor "IF" but we can make a notation for it. *)
     instruction (a ::: list_ a ::: A) B ->
     instruction A B ->
     instruction (list_ a :: A) B
-| MAP_list_body {elt b A} :
-    instruction (elt ::: A) (b ::: A) ->
-    instruction (list_ elt ::: A) (list_ b ::: A)
-| ITER_list {elt A} : instruction (elt :: A) A -> instruction (list_ elt :: A) A
 | CREATE_CONTRACT {p g S} :
     instruction
       (key_hash ::: option_ key_hash ::: bool ::: bool ::: mutez :::
@@ -831,7 +407,7 @@ this constructor "IF" but we can make a notation for it. *)
 | SOURCE {S} : instruction S (address :: S)
 | SENDER {S} : instruction S (address :: S)
 | SELF {p S} : instruction S (contract p :: S)
-(* p should be obtained from the node *)
+(* p should be the current parameter type *)
 | AMOUNT {S} : instruction S (mutez ::: S)
 | IMPLICIT_ACCOUNT {S} : instruction (key_hash ::: S) (contract unit :: S)
 | STEPS_TO_QUOTA {S} : instruction S (nat ::: S)
@@ -842,25 +418,52 @@ this constructor "IF" but we can make a notation for it. *)
 | BLAKE2B {S} : instruction (bytes ::: S) (bytes ::: S)
 | SHA256 {S} : instruction (bytes ::: S) (bytes ::: S)
 | SHA512 {S} : instruction (bytes ::: S) (bytes ::: S)
-| CHECK_SIGNATURE {S} : instruction (key ::: signature ::: bytes ::: S) (bool ::: S).
+| CHECK_SIGNATURE {S} : instruction (key ::: signature ::: bytes ::: S) (bool ::: S)
 
+with
+concrete_data : type -> Set :=
+| Int_constant : Z -> concrete_data int
+| Nat_constant : N -> concrete_data nat
+| String_constant : String.string -> concrete_data string
+| Timestamp_constant : Z -> concrete_data timestamp
+| Signature_constant : String.string -> concrete_data signature
+| Key_constant : String.string -> concrete_data key
+| Key_hash_constant : String.string -> concrete_data key_hash
+| Mutez_constant : mutez_constant -> concrete_data mutez
+| Contract_constant {a} : forall cst : contract_constant,
+    get_contract_type cst = Return _ a -> concrete_data (contract a)
+| Unit : concrete_data unit
+| True_ : concrete_data bool
+| False_ : concrete_data bool
+| Pair {a b : type} : concrete_data a -> concrete_data b -> concrete_data (pair a b)
+| Left {a b : type} : concrete_data a -> concrete_data (or a b)
+| Right {a b : type} : concrete_data b -> concrete_data (or a b)
+| Some_ {a : type} : concrete_data a -> concrete_data (option_ a)
+| None_ {a : type} : concrete_data (option_ a)
+
+(* Commented because not documented *)
+(* | Concrete_list {a} : Datatypes.list (concrete_data a) -> concrete_data (list_ a) *)
+| Concrete_set {a : comparable_type} :
+    Datatypes.list (concrete_data a) -> concrete_data (set_ a)
+| Concrete_map {a : comparable_type} {b} :
+    Datatypes.list (elt_pair (concrete_data a) (concrete_data b)) ->
+    concrete_data (map a b)
+| Instruction {a b} : instruction (a ::: nil) (b ::: nil) ->
+                      concrete_data (lambda a b).
 (* TODO: add the no-ops CAST and RENAME *)
 
-Notation "'IF'" := (IF_).
 
-Definition stack_type := list type.
-
-Fixpoint stack (t : stack_type) : Set :=
-  match t with
-  | nil => Datatypes.unit
-  | cons a A => data a * stack A
-  end.
-
+Coercion int_constant := Int_constant.
+Coercion nat_constant := Nat_constant.
+Coercion string_constant := String_constant.
 
 Definition full_contract params storage :=
   instruction ((pair params storage) ::: nil) ((pair (list_ operation) storage) ::: nil).
 
 End syntax.
+
+Notation "'IF'" := (IF_).
+Definition stack_type := list type.
 
 Notation "A ;; B" := (SEQ A B) (at level 100, right associativity).
 
