src/semantics.v
@@ -10,7 +10,329 @@ Import syntax.
 
 Section semantics.
 
-  Parameter nd : node.
+  Context {get_contract_type : contract_constant -> M type}.
+
+  Implicit Types (get_contract_type : contract_constant -> M type).
+
+  Fixpoint data (a : type) {struct a} : Set :=
+    match a with
+    | Comparable_type b => comparable_data b
+    | address => address_constant
+    | signature => signature_constant
+    | operation => operation_constant
+    | key => key_constant
+    | unit => Datatypes.unit
+    | pair a b => data a * data b
+    | or a b => sum (data a) (data b)
+    | option_ a => option (data a)
+    | list_ a => list (data a)
+    | set_ a => set.set (comparable_data a) (compare a)
+    | map a b => map.map (comparable_data a) (data b) (compare a)
+    | big_map a b => map.map (comparable_data a) (data b) (compare a)
+    | lambda a b => @instruction get_contract_type (a ::: nil) (b ::: nil)
+    | contract a => {s : contract_constant | get_contract_type s = Return _ a }
+    end.
+
+  Record node : Set :=
+    mk_node
+      {
+        create_contract : forall g p,
+          comparable_data key_hash ->
+          option (comparable_data key_hash) ->
+          Datatypes.bool -> Datatypes.bool -> tez.mutez ->
+          data (lambda (pair p g) (pair (list_ operation) g)) ->
+          data g -> M (data (pair operation address));
+        create_account :
+          comparable_data key_hash ->
+          option (comparable_data key_hash) ->
+          Datatypes.bool -> tez.mutez ->
+          M (data operation * data (contract unit));
+        transfer_tokens : forall p,
+            data p -> tez.mutez -> data (contract p) ->
+            M (data operation);
+        set_delegate : option (comparable_data key_hash) ->
+                       M (data operation);
+        balance : M tez.mutez;
+        address_ : forall p, data (contract p) -> M (data address);
+        contract_ : forall p, data address -> M (option (data (contract p)));
+        source : M (data address);
+        sender : M (data address);
+        self : forall p, M (data (contract p));
+        amount : M tez.mutez;
+        implicit_account :
+          comparable_data key_hash -> M (data (contract unit));
+        steps_to_quota : M N;
+        now : M (comparable_data timestamp);
+        hash_key : data key -> M (comparable_data key_hash);
+        pack : forall a, data a -> M str;
+        unpack : forall a, str -> M (option (data a));
+        blake2b : str -> M str;
+        sha256 : str -> M str;
+        sha512 : str -> M str;
+        check_signature :
+          data key -> data signature -> String.string -> M Datatypes.bool;
+        read_contract_constant a : forall cst : contract_constant,
+            get_contract_type cst = Return _ a -> M (data (contract a))
+      }.
+
+  Variable nd : node.
+
+  Fixpoint stack (t : stack_type) : Set :=
+    match t with
+    | nil => Datatypes.unit
+    | cons a A => data a * stack A
+    end.
+
+
+
+  Fixpoint concrete_data_to_data (a : type) (d : concrete_data a) : data a :=
+    match d with
+    | Int_constant x => x
+    | Nat_constant x => x
+    | String_constant x => x
+    | Timestamp_constant x => x
+    | Signature_constant x => Mk_sig x
+    | Key_constant x => Mk_key x
+    | Key_hash_constant x => Mk_key_hash x
+    | Mutez_constant (Mk_mutez x) => x
+    | @Contract_constant _ a x H => exist _ x H
+    | Unit => tt
+    | True_ => true
+    | False_ => false
+    | Pair a b => (concrete_data_to_data _ a, concrete_data_to_data _ b)
+    | Left a => inl (concrete_data_to_data _ a)
+    | Right b => inr (concrete_data_to_data _ b)
+    | Some_ a => Some (concrete_data_to_data _ a)
+    | None_ => None
+    | @Concrete_set _ a l =>
+      (fix concrete_data_set_to_data (l : list (concrete_data a)) :=
+         match l with
+         | nil => set.empty _ _
+         | cons x l =>
+           set.insert
+             (data a)
+             (comparable.compare a)
+             (comparable.compare_eq_iff a)
+             (comparable.lt_trans a)
+             (comparable.gt_trans a)
+             (concrete_data_to_data a x)
+             (concrete_data_set_to_data l)
+         end) l
+    | @Concrete_map _ a b l =>
+      (fix concrete_data_map_to_data
+           (l : Datatypes.list (elt_pair (concrete_data a) (concrete_data b))) :=
+         match l with
+         | nil => map.empty _ _ _
+         | cons (Elt _ _ x y) l =>
+           map.update
+             (data a)
+             (data b)
+             (comparable.compare a)
+             (comparable.compare_eq_iff a)
+             (comparable.lt_trans a)
+             (comparable.gt_trans a)
+             (concrete_data_to_data _ x)
+             (Some (concrete_data_to_data _ y))
+             (concrete_data_map_to_data l)
+         end) l
+    | Instruction i => i
+    end.
+
+  Definition or_fun a (v : bitwise_variant a) : data a -> data a -> data a :=
+    match v with
+    | Bitwise_variant_bool => orb
+    | Bitwise_variant_nat => N.lor
+    end.
+
+  Definition and a (v : bitwise_variant a) : data a -> data a -> data a :=
+    match v with
+    | Bitwise_variant_bool => andb
+    | Bitwise_variant_nat => N.land
+    end.
+
+  Definition xor a (v : bitwise_variant a) : data a -> data a -> data a :=
+    match v with
+    | Bitwise_variant_bool => xorb
+    | Bitwise_variant_nat => N.lxor
+    end.
+
+  Definition not a b (v : not_variant a b) : data a -> data b :=
+    match v with
+    | Not_variant_bool => negb
+    | Not_variant_int => fun x => (- 1 - x)%Z
+    | Not_variant_nat => fun x => (- 1 - Z.of_N x)%Z
+    end.
+
+  Definition neg a (v : neg_variant a) : data a -> data int :=
+    match v with
+    | Neg_variant_nat => fun x => (- Z.of_N x)%Z
+    | Neg_variant_int => fun x => (- x)%Z
+    end.
+
+  Definition add a b c (v : add_variant a b c) : data a -> data b -> M (data c) :=
+    match v with
+    | Add_variant_nat_nat => fun x y => Return _ (x + y)%N
+    | Add_variant_nat_int => fun x y => Return _ (Z.of_N x + y)%Z
+    | Add_variant_int_nat => fun x y => Return _ (x + Z.of_N y)%Z
+    | Add_variant_int_int => fun x y => Return _ (x + y)%Z
+    | Add_variant_timestamp_int => fun x y => Return _ (x + y)%Z
+    | Add_variant_int_timestamp => fun x y => Return _ (x + y)%Z
+    | Add_variant_tez_tez =>
+      fun x y => tez.of_Z (tez.to_Z x + tez.to_Z y)
+    end.
+
+
+  Definition sub a b c (v : sub_variant a b c) : data a -> data b -> M (data c) :=
+    match v with
+    | Sub_variant_nat_nat => fun x y => Return _ (Z.of_N x - Z.of_N y)%Z
+    | Sub_variant_nat_int => fun x y => Return _ (Z.of_N x - y)%Z
+    | Sub_variant_int_nat => fun x y => Return _ (x - Z.of_N y)%Z
+    | Sub_variant_int_int => fun x y => Return _ (x - y)%Z
+    | Sub_variant_timestamp_int => fun x y => Return _ (x - y)%Z
+    | Sub_variant_timestamp_timestamp => fun x y => Return _ (x - y)%Z
+    | Sub_variant_tez_tez => fun x y => tez.of_Z (tez.to_Z x - tez.to_Z y)
+    end.
+
+  Definition mul a b c (v : mul_variant a b c) : data a -> data b -> M (data c) :=
+    match v with
+    | Mul_variant_nat_nat => fun x y => Return _ (x * y)%N
+    | Mul_variant_nat_int => fun x y => Return _ (Z.of_N x * y)%Z
+    | Mul_variant_int_nat => fun x y => Return _ (x * Z.of_N y)%Z
+    | Mul_variant_int_int => fun x y => Return _ (x * y)%Z
+    | Mul_variant_tez_nat => fun x y => tez.of_Z (tez.to_Z x * Z.of_N y)
+    | Mul_variant_nat_tez => fun x y => tez.of_Z (Z.of_N x * tez.to_Z y)
+    end.
+
+  Definition ediv_Z x y :=
+    if (y =? 0)%Z then None else Some (x / y, Z.to_N (x mod y))%Z.
+  Definition ediv_N x y :=
+    if (y =? 0)%N then None else Some (x / y, x mod y)%N.
+
+  Definition ediv a b c d (v : ediv_variant a b c d) : data a -> data b -> data (option_ (pair c d)) :=
+    match v with
+    | Ediv_variant_nat_nat => fun x y => ediv_N x y
+    | Ediv_variant_nat_int => fun x y => ediv_Z (Z.of_N x) y
+    | Ediv_variant_int_nat => fun x y => ediv_Z x (Z.of_N y)
+    | Ediv_variant_int_int => fun x y => ediv_Z x y
+    | Ediv_variant_tez_nat =>
+      fun x y =>
+        match ediv_Z (tez.to_Z x) (Z.of_N y) with
+        | None => None
+        | Some (quo, rem) =>
+          match tez.of_Z quo, tez.of_Z (Z.of_N rem) with
+          | Return _ quo, Return _ rem => Some (quo, rem)
+          | _, _ => None
+          end
+        end
+    | Ediv_variant_tez_tez =>
+      fun x y =>
+        match ediv_Z (tez.to_Z x) (tez.to_Z y) with
+        | None => None
+        | Some (quo, rem) =>
+          match tez.of_Z (Z.of_N rem) with
+          | Return _ rem => Some (Z.to_N quo, rem)
+          | _ => None
+          end
+        end
+    end.
+
+  Definition concat a (v : stringlike_variant a) : data a -> data a -> data a :=
+    match v with
+    | Stringlike_variant_string => String.append
+    | Stringlike_variant_bytes => String.append
+    end.
+
+  Definition slice a (v : stringlike_variant a) : data nat -> data nat -> data a -> data (option_ a) :=
+    match v with
+    | Stringlike_variant_string =>
+      fun (n1 n2 : N) (s : data string) =>
+        if (n1 + n2 <=? N.of_nat (String.length s))%N then
+          (Some (String.substring (N.to_nat n1) (N.to_nat n2) s)
+           : data (option_ string))
+        else None
+    | Stringlike_variant_bytes =>
+      fun n1 n2 s =>
+        if (n1 + n2 <=? N.of_nat (String.length s))%N then
+          Some (String.substring (N.to_nat n1) (N.to_nat n2) s)
+        else None
+    end.
+
+  Definition mem a b (v : mem_variant a b) : data a -> data b -> data bool :=
+    match v with
+    | Mem_variant_set a =>
+      fun (x : data a) (y : data (set_ a)) => set.mem _ _ (compare_eq_iff a) x y
+    | Mem_variant_map _ _ => map.mem _ _ _
+    | Mem_variant_bigmap _ _ => map.mem _ _ _
+    end.
+
+  Definition update a b c (v : update_variant a b c) :
+    data a -> data b -> data c -> data c :=
+    match v with
+    | Update_variant_set a =>
+      set.update _ _ (compare_eq_iff a) (lt_trans a) (gt_trans a)
+    | Update_variant_map k v =>
+      map.update _ _ _ (compare_eq_iff k) (lt_trans k) (gt_trans k)
+    | Update_variant_bigmap k _ =>
+      map.update _ _ _ (compare_eq_iff k) (lt_trans k) (gt_trans k)
+    end.
+
+  Definition size a (v : size_variant a) : data a -> Datatypes.nat :=
+    match v with
+    | Size_variant_list a => fun l => List.length l
+    | Size_variant_set a => set.size (data a) (compare a)
+    | Size_variant_map k v => map.size (data k) (data v) (compare k)
+    | Size_variant_string => String.length
+    | Size_variant_bytes => String.length
+    end.
+
+  Definition iter_destruct a b (v : iter_variant a b)
+    : data b -> data (option_ (pair a b)) :=
+    match v with
+    | Iter_variant_set _ => set.destruct _ _
+    | Iter_variant_map _ _ => set.destruct _ _
+    | Iter_variant_list _ =>
+      fun l => match l with
+               | nil => None
+               | cons a l => Some (a, l)
+               end
+    end.
+
+  Definition get k val c (v : get_variant k val c)
+    : data k -> data c -> data (option_ val) :=
+    match v with
+    | Get_variant_map _ _ => map.get _ _ _
+    | Get_variant_bigmap _ _ => map.get _ _ _
+    end.
+
+  Definition map_destruct a b ca cb (v : map_variant a b ca cb)
+    : data ca -> data (option_ (pair a ca)) :=
+    match v with
+    | Map_variant_map _ _ _ => set.destruct _ _
+    | Map_variant_list _ _ =>
+      fun l => match l with
+               | nil => None
+               | cons a l => Some (a, l)
+               end
+    end.
+
+  Definition map_empty a b ca cb (v : map_variant a b ca cb)
+    : data cb :=
+    match v with
+    | Map_variant_map _ _ _ => map.empty _ _ _
+    | Map_variant_list _ _ => nil
+    end.
+
+  Definition map_insert a b ca cb (v : map_variant a b ca cb)
+    : data a -> data b -> data cb -> data cb :=
+    match v with
+    | Map_variant_map k_ty _ v_ty =>
+      fun '(k, _) v (m : data (map k_ty v_ty)) =>
+        map.update _ _ _ (comparable.compare_eq_iff _) (comparable.lt_trans _) (comparable.gt_trans _) k (Some v) m
+    | Map_variant_list _ _ =>
+      fun _ => cons
+    end.
+
+
 
   (* The gas argument is used to ensure termination, it is not the
   amount of gas that is actually required to run the contract because
@@ -22,10 +344,8 @@ Section semantics.
     | O => fun SA => Failed _ Out_of_fuel
     | S n =>
       match i in instruction A B return stack A -> M (stack B) with
-      | @FAILWITH A B a =>
-        fun xS =>
-          let (x, S) := xS in
-          Failed _ (Assertion_Failure (data a) x)
+      | @FAILWITH _ A B a =>
+        fun '(x, _) => Failed _ (Assertion_Failure (data a) x)
 
       (* According to the documentation, FAILWITH's argument should
          not be part of the state reached by the instruction but the
@@ -36,420 +356,180 @@ Section semantics.
       | SEQ B C =>
         fun SA => bind (eval C n) (eval B n SA)
       | IF_ bt bf =>
-        fun SbA =>
-          let (b, SA) := SbA in
-          if b then eval bt n SA else eval bf n SA
+        fun '(b, SA) => if b then eval bt n SA else eval bf n SA
       | LOOP body =>
-        fun SbA =>
-          let (b, SA) := SbA in
-          if b then eval (SEQ body (LOOP body)) n SA else Return _ SA
+        fun '(b, SA) => if b then eval (body;; (LOOP body)) n SA else Return _ SA
       | LOOP_LEFT body =>
-        fun SabA =>
-          let (ab, SA) := SabA in
+        fun '(ab, SA) =>
           match ab return M (stack (_ ::: _)) with
-          | inl x => eval (SEQ body (LOOP_LEFT body)) n (x, SA)
+          | inl x => eval (body;; LOOP_LEFT body) n (x, SA)
           | inr y => Return _ (y, SA)
           end
       | DIP i =>
-        fun SbA =>
-          let (y, SA) := SbA in
-          bind (fun SC => Return _ (y, SC)) (eval i n SA)
+        fun '(y, SA) => bind (fun SC => Return _ (y, SC)) (eval i n SA)
       | EXEC =>
-        fun SxfA =>
-          match SxfA return M (stack (_ ::: _)) with
-          | (x, (f, SA)) =>
-            bind (fun y =>
-                    Return _ (y, SA))
-                 (f x)
-          end
-      | DROP =>
-        fun SxA =>
-          let (x, SA) := SxA in
-          Return _ SA
-      | DUP =>
-        fun SxA =>
-          let (x, SA) := SxA in
-          Return _ (x, (x, SA))
-      | SWAP =>
-        fun SxyA =>
-          let (x, SyA) := SxyA in
-          let (y, SA) := SyA in
-          Return _ (y, (x, SA))
-      | PUSH a x => fun SA => Return _ (x, SA)
+        fun '(x, (f, SA)) =>
+          bind (fun '(y, tt) => Return _ (y, SA)) (eval f n (x, tt))
+      | DROP => fun '(_, SA) => Return _ SA
+      | DUP => fun '(x, SA) => Return _ (x, (x, SA))
+      | SWAP => fun '(x, (y, SA)) => Return _ (y, (x, SA))
+      | PUSH a x => fun SA => Return _ (concrete_data_to_data _ x, SA)
       | UNIT => fun SA => Return _ (tt, SA)
-      | LAMBDA a b code =>
-        fun SA =>
-          Return _ (fun x : data a =>
-                       @bind
-                         (stack (b ::: nil))
-                         (data b)
-                         (fun SB =>
-                            let (y, tt) := SB in
-                            Return _ y)
-                         (eval code n (x, tt)), SA)
-      | EQ =>
-        fun SxA =>
-          let (x, SA) := SxA in
-          Return _ ((x =? 0)%Z, SA)
-      | NEQ =>
-        fun SxA =>
-          let (x, SA) := SxA in
-          Return _ (negb (x =? 0)%Z, SA)
-      | LT =>
-        fun SxA =>
-          let (x, SA) := SxA in
-          Return _ ((x <? 0)%Z, SA)
-      | GT =>
-        fun SxA =>
-          let (x, SA) := SxA in
-          Return _ ((x >? 0)%Z, SA)
-      | LE =>
-        fun SxA =>
-          let (x, SA) := SxA in
-          Return _ ((x <=? 0)%Z, SA)
-      | GE =>
-        fun SxA =>
-          let (x, SA) := SxA in
-          Return _ ((x >=? 0)%Z, SA)
-      | @OR b s _ =>
-        fun SxyA =>
-          let (x, SyA) := SxyA in
-          let (y, SA) := SyA in
+      | LAMBDA a b code => fun SA => Return _ (code, SA)
+      | EQ => fun '(x, SA) => Return _ ((x =? 0)%Z, SA)
+      | NEQ => fun '(x, SA) => Return _ (negb (x =? 0)%Z, SA)
+      | LT => fun '(x, SA) => Return _ ((x <? 0)%Z, SA)
+      | GT => fun '(x, SA) => Return _ ((x >? 0)%Z, SA)
+      | LE => fun '(x, SA) => Return _ ((x <=? 0)%Z, SA)
+      | GE => fun '(x, SA) => Return _ ((x >=? 0)%Z, SA)
+      | @OR _ _ s =>
+        fun '(x, (y, SA)) => Return _ (or_fun _ (bitwise_variant_field _ s) x y, SA)
+      | @AND _ _ s =>
+        fun '(x, (y, SA)) => Return _ (and _ (bitwise_variant_field _ s) x y, SA)
+      | @XOR _ _ s =>
+        fun '(x, (y, SA)) => Return _ (xor _ (bitwise_variant_field _ s) x y, SA)
+      | @NOT _ _ s =>
+        fun '(x, SA) => Return _ (not _ _ (not_variant_field _ s) x, SA)
+      | @NEG _ _ s =>
+        fun '(x, SA) => Return _ (neg _ (neg_variant_field _ s) x, SA)
+      | ABS => fun '(x, SA) => Return _ (Z.abs_N x, SA)
+      | @ADD _ _ _ s =>
+        fun '(x, (y, SA)) =>
           bind (fun r => Return _ (r, SA))
-               (@bitwise.or b s x y)
-      | @AND b s _ =>
-        fun SxyA =>
-          let (x, SyA) := SxyA in
-          let (y, SA) := SyA in
+               (add _ _ _ (add_variant_field _ _ s) x y)
+      | @SUB _ _ _ s =>
+        fun '(x, (y, SA)) =>
           bind (fun r => Return _ (r, SA))
-               (@bitwise.and b s x y)
-      | @XOR b s _ =>
-        fun SxyA =>
-          let (x, SyA) := SxyA in
-          let (y, SA) := SyA in
+               (sub _ _ _ (sub_variant_field _ _ s) x y)
+      | @MUL _ _ _ s =>
+        fun '(x, (y, SA)) =>
           bind (fun r => Return _ (r, SA))
-               (@bitwise.xor b s x y)
-      | NOT =>
-        fun SxA =>
-          let (x, SA) := SxA in
-          bind (fun r => Return _ (r, SA))
-               (not.not _ x)
-      | @NEG b s _ =>
-        fun SxA =>
-          let (x, SA) := SxA in
-          bind (fun r => Return _ (r, SA))
-               (@neg.op b s x)
-      | ABS =>
-        fun SxA =>
-          let (x, SA) := SxA in
-          Return _ (Z.abs_N x, SA)
-      | ADD =>
-        fun SxyA =>
-          let (x, SyA) := SxyA in
-          let (y, SA) := SyA in
-          bind (fun r => Return _ (r, SA))
-               (add.op _ _ x y)
-      | SUB =>
-        fun SxyA =>
-          let (x, SyA) := SxyA in
-          let (y, SA) := SyA in
-          bind (fun r => Return _ (r, SA))
-               (sub.op _ _ x y)
-      | MUL =>
-        fun SxyA =>
-          let (x, SyA) := SxyA in
-          let (y, SA) := SyA in
-          bind (fun r => Return _ (r, SA))
-               (mul.op _ _ x y)
-      | EDIV =>
-        fun SxyA =>
-          let (x, SyA) := SxyA in
-          let (y, SA) := SyA in
-          bind (fun r => Return _ (r, SA))
-               (ediv.op _ _ x y)
-      | LSL =>
-        fun SxyA =>
-          let (x, SyA) := SxyA in
-          let (y, SA) := SyA in
-          Return _ (N.shiftl x y, SA)
-      | LSR =>
-        fun SxyA =>
-          let (x, SyA) := SxyA in
-          let (y, SA) := SyA in
-          Return _ (N.shiftr x y, SA)
+               (mul _ _ _ (mul_variant_field _ _ s) x y)
+      | @EDIV _ _ _ s =>
+        fun '(x, (y, SA)) =>
+          Return _ (ediv _ _ _ _ (ediv_variant_field _ _ s) x y, SA)
+      | LSL => fun '(x, (y, SA)) => Return _ (N.shiftl x y, SA)
+      | LSR => fun '(x, (y, SA)) => Return _ (N.shiftr x y, SA)
       | COMPARE =>
-        fun SxyA =>
-          let (x, SyA) := SxyA in
-          let (y, SA) := SyA in
-          Return _ (comparison_to_int (compare _ x y), SA)
-      | @CONCAT _ _ i =>
-        fun SxyA =>
-          let (x, SyA) := SxyA in
-          let (y, SA) := SyA in
-          bind (fun r => Return _ (r, SA))
-               (@string_like.concat _ i x y)
+        fun '(x, (y, SA)) => Return _ (comparison_to_int (compare _ x y), SA)
+      | @CONCAT _ _ s =>
+        fun '(x, (y, SA)) =>
+          Return _ (concat _ (stringlike_variant_field _ s) x y, SA)
       | @SLICE _ _ i =>
-        fun SabcA =>
-          match SabcA with
-            (a, (b, (c, SA))) =>
-            bind (fun r => Return _ (r, SA))
-                 (@string_like.slice _ i a b c)
-          end
-      | PAIR =>
-        fun SxyA =>
-          let (x, SyA) := SxyA in
-          let (y, SA) := SyA in
-          Return _ ((x, y), SA)
-      | CAR =>
-        fun SxyA =>
-          let (xy, SA) := SxyA in
-          let (x, y) := xy in
-          Return _ (x, SA)
-      | CDR =>
-        fun SxyA =>
-          let (xy, SA) := SxyA in
-          let (x, y) := xy in
-          Return _ (y, SA)
-      | EMPTY_SET a =>
-        fun SA => Return _ (set.empty _ (compare a), SA)
-      | MEM =>
-        fun SxyA =>
-          let (x, SyA) := SxyA in
-          let (y, SA) := SyA in
-          bind (fun r => Return _ (r, SA))
-               (mem.op _ _ _ x y)
-      | UPDATE =>
-        fun SxyzA =>
-          let (x, SyzA) := SxyzA in
-          let (y, SzA) := SyzA in
-          let (z, SA) := SzA in
-          bind (fun r => Return _ (r, SA))
-               (update.op _ _ _ x y z)
-      | ITER_set body =>
-        fun SxA =>
-          let (x, SA) := SxA in
-          match set.destruct _ _ x with
+        fun '(n1, (n2, (s, SA))) =>
+          Return _ (slice _ (stringlike_variant_field _ i) n1 n2 s, SA)
+      | PAIR => fun '(x, (y, SA)) => Return _ ((x, y), SA)
+      | CAR => fun '((x, y), SA) => Return _ (x, SA)
+      | CDR => fun '((x, y), SA) => Return _ (y, SA)
+      | EMPTY_SET a => fun SA => Return _ (set.empty _ (compare a), SA)
+      | @MEM _ _ _ s =>
+        fun '(x, (y, SA)) =>
+          Return _ (mem _ _ (mem_variant_field _ _ s) x y, SA)
+      | @UPDATE _ _ _ _ s =>
+        fun '(x, (y, (z, SA))) =>
+          Return _ (update _ _ _ (update_variant_field _ _ _ s) x y z, SA)
+      | @ITER _ _ s _ body =>
+        fun '(x, SA) =>
+          match iter_destruct _ _ (iter_variant_field _ s) x with
           | None => Return _ SA
           | Some (a, y) =>
             bind (fun SB =>
-                    eval (ITER_set body) n (y, SB))
+                    eval (ITER body) n (y, SB))
                  (eval body n (a, SA))
           end
-      | SIZE =>
-        fun SxA =>
-          let (x, SA) := SxA in
-          bind (fun r => Return _ (r, SA))
-               (@size.op data _ x)
+      | @SIZE _ _ s =>
+        fun '(x, SA) => Return _ (N.of_nat (size _ (size_variant_field _ s) x), SA)
       | EMPTY_MAP k val =>
         fun SA => Return _ (map.empty (comparable_data k) (data val) _, SA)
-      | GET =>
-        fun SxyA =>
-          let (x, SyA) := SxyA in
-          let (y, SA) := SyA in
-          bind (fun r => Return _ (r, SA))
-               (get.op _ _ _ x y)
-      | MAP_map_body body =>
-        fun SxA =>
-          let (x, SA) := SxA in
-          match set.destruct _ _ x with
-          | None => Return _ (map.empty _ _ _, SA)
+      | @GET _ _ _ s =>
+        fun '(x, (y, SA)) =>
+          Return _ (get _ _ _ (get_variant_field _ _ s) x y, SA)
+      | @MAP _ _ _ s _ body =>
+        let v := (map_variant_field _ _ s) in
+        fun '(x, SA) =>
+          match map_destruct _ _ _ _ v x with
+          | None => Return _ (map_empty _ _ _ _ v, SA)
           | Some (a, y) =>
-            let (k, _) := a in
-            bind (fun SbB : data _ * _ =>
-                    let (b, SB) := SbB in
-                    bind (fun ScC : data (map _ _) * _ =>
-                            let (c, SC) := ScC in
-                            Return _ (map.update _ _ _ (compare_eq_iff _) (lt_trans _) (gt_trans _) k (Some b) c, SC))
-                         (eval (MAP_map_body body) n (y, SB)))
+            bind (fun '(b, SB) =>
+                    bind (fun '(c, SC) =>
+                            Return _ (map_insert _ _ _ _ v a b c,
+                                      SC))
+                         (eval (MAP body) n (y, SB)))
                  (eval body n (a, SA))
           end
-      | ITER_map body =>
-        fun SxA =>
-          let (x, SA) := SxA in
-          match set.destruct _ _ x with
-          | None => Return _ SA
-          | Some (a, y) =>
-            bind (fun SB =>
-                    eval (ITER_map body) n (y, SB))
-                 (eval body n (a, SA))
-          end
-      | SOME =>
-        fun SxA =>
-          let (x, SA) := SxA in
-          Return _ (Some x, SA)
-      | NONE _ =>
-        fun SA =>
-          Return _ (None, SA)
+      | SOME => fun '(x, SA) => Return _ (Some x, SA)
+      | NONE _ => fun SA => Return _ (None, SA)
       | IF_NONE bt bf =>
-        fun SbA =>
-          match SbA with
-          | (None, SA) => eval bt n SA
-          | (Some b, SA) => eval bf n (b, SA)
+        fun '(b, SA) =>
+          match b with
+          | None => eval bt n SA
+          | Some b => eval bf n (b, SA)
           end
-      | LEFT _ =>
-        fun SxA =>
-          let (x, SA) := SxA in
-          Return _ (inl x, SA)
-      | RIGHT _ =>
-        fun SxA =>
-          let (x, SA) := SxA in
-          Return _ (inr x, SA)
+      | LEFT _ => fun '(x, SA) => Return _ (inl x, SA)
+      | RIGHT _ => fun '(x, SA) => Return _ (inr x, SA)
       | IF_LEFT bt bf =>
-        fun SbA =>
-          match SbA with
-          | (inl a, SA) => eval bt n (a, SA)
-          | (inr b, SA) => eval bf n (b, SA)
+        fun '(b, SA) =>
+          match b with
+          | inl a => eval bt n (a, SA)
+          | inr b => eval bf n (b, SA)
           end
       | IF_RIGHT bt bf =>
-        fun SbA =>
-          match SbA with
-          | (inl a, SA) => eval bf n (a, SA)
-          | (inr b, SA) => eval bt n (b, SA)
+        fun '(b, SA) =>
+          match b with
+          | inl a => eval bf n (a, SA)
+          | inr b => eval bt n (b, SA)
           end
-      | CONS =>
-        fun SxyA =>
-          let (x, SyA) := SxyA in
-          let (y, SA) := SyA in
-          Return _ (cons x y, SA)
-      | NIL _ =>
-        fun SA =>
-          Return _ (nil, SA)
+      | CONS => fun '(x, (y, SA)) => Return _ (cons x y, SA)
+      | NIL _ => fun SA => Return _ (nil, SA)
       | IF_CONS bt bf =>
-        fun SbA =>
-          match SbA with
-          | (cons a b, SA) => eval bt n (a, (b, SA))
-          | (nil, SA) => eval bf n SA
-          end
-      | MAP_list_body body =>
-        fun SxA =>
-          let (x, SA) := SxA in
-          match x with
-          | nil => Return _ (nil, SA)
-          | cons a y =>
-            bind (fun SbB : data _ * _ =>
-                    let (b, SB) := SbB in
-                    bind (fun ScC : data (list_ _) * _ =>
-                            let (c, SC) := ScC in
-                            Return _ (cons b c, SC))
-                         (eval (MAP_list_body body) n (y, SB)))
-                 (eval body n (a, SA))
-          end
-      | ITER_list body =>
-        fun SxA =>
-          let (x, SA) := SxA in
-          match x with
-          | nil => Return _ SA
-          | cons a y =>
-            bind (fun SB =>
-                    eval (ITER_list body) n (y, SB))
-                 (eval body n (a, SA))
+        fun '(l, SA) =>
+          match l with
+          | cons a b => eval bt n (a, (b, SA))
+          | nil => eval bf n SA
           end
       | CREATE_CONTRACT =>
-        fun SabcdefgA =>
-          match SabcdefgA with
-          | (a, (b, (c, (d, (e, (f, (g, SA))))))) =>
-            bind (fun r : data operation * data address =>
-                    let (a, b) := r in Return _ (a, (b, SA)))
-                 (create_contract nd _ _ a b c d e f g)
-          end
+        fun '(a, (b, (c, (d, (e, (f, (g, SA))))))) =>
+          bind (fun '(a, b) => Return _ (a, (b, SA)))
+               (create_contract nd _ _ a b c d e f g)
       | CREATE_CONTRACT_literal _ _ f =>
-        fun SabcdegA =>
-          let ff := fun p =>
-                      bind (fun SxA =>
-                              match SxA with (x, tt) => Return _ x end)
-                           (eval f n (p, tt))
-          in
-          match SabcdegA with
-          | (a, (b, (c, (d, (e, (g, SA)))))) =>
-            bind (fun r : data operation * data address =>
-                     let (a, b) := r in Return _ (a, (b, SA)))
-                 (create_contract nd _ _ a b c d e ff g)
-          end
+        fun '(a, (b, (c, (d, (e, (g, SA)))))) =>
+          bind (fun '(a, b) => Return _ (a, (b, SA)))
+               (create_contract nd _ _ a b c d e f g)
       | CREATE_ACCOUNT =>
-        fun SabcdA =>
-          match SabcdA with
-          | (a, (b, (c, (d, SA)))) =>
-            bind (fun r : data _ * data _ =>
-                     let (a, b) := r in Return _ (a, (b, SA)))
-                 (create_account nd a b c d)
-          end
+        fun '(a, (b, (c, (d, SA)))) =>
+          bind (fun '(a, b) => Return _ (a, (b, SA)))
+               (create_account nd a b c d)
       | TRANSFER_TOKENS =>
-        fun SabcdA =>
-          match SabcdA with
-          | (a, (b, (c, SA))) =>
-            bind (fun r => Return _ (r, SA))
-                 (transfer_tokens nd _ a b c)
-          end
+        fun '(a, (b, (c, SA))) =>
+          bind (fun r => Return _ (r, SA))
+               (transfer_tokens nd _ a b c)
       | SET_DELEGATE =>
-        fun SxA =>
-          let (x, SA) := SxA in
+        fun '(x, SA) =>
           bind (fun r => Return _ (r, SA))
                (set_delegate nd x)
       | BALANCE => fun SA => bind (fun r => Return _ (r, SA)) (balance nd)
       | ADDRESS =>
-        fun SxA =>
-          let (x, SA) := SxA in
-          bind (fun r => Return _ (r, SA))
-               (address_ nd _ x)
+        fun '(x, SA) => bind (fun r => Return _ (r, SA)) (address_ nd _ x)
       | CONTRACT _ =>
-        fun SxA =>
-          let (x, SA) := SxA in
-          bind (fun r => Return _ (r, SA))
-               (contract_ nd _ x)
-      | SOURCE =>
-        fun SA =>
-          bind (fun r => Return _ (r, SA))
-               (source nd)
-      | SENDER =>
-        fun SA =>
-          bind (fun r => Return _ (r, SA))
-               (sender nd)
-      | SELF =>
-        fun SA =>
-          bind (fun r => Return _ (r, SA))
-               (self nd _)
+        fun '(x, SA) => bind (fun r => Return _ (r, SA)) (contract_ nd _ x)
+      | SOURCE => fun SA => bind (fun r => Return _ (r, SA)) (source nd)
+      | SENDER => fun SA => bind (fun r => Return _ (r, SA)) (sender nd)
+      | SELF => fun SA => bind (fun r => Return _ (r, SA)) (self nd _)
       | AMOUNT => fun SA => bind (fun r => Return _ (r, SA)) (amount nd)
       | IMPLICIT_ACCOUNT =>
-        fun SxA =>
-          let (x, SA) := SxA in
-          bind (fun r => Return _ (r, SA))
-               (implicit_account nd x)
+        fun '(x, SA) => bind (fun r => Return _ (r, SA)) (implicit_account nd x)
       | STEPS_TO_QUOTA =>
-        fun SA =>
-          bind (fun r => Return _ (r, SA))
-               (steps_to_quota nd)
+        fun SA => bind (fun r => Return _ (r, SA)) (steps_to_quota nd)
       | NOW => fun SA => bind (fun r => Return _ (r, SA)) (now nd)
-      | PACK => fun SxA => let (x, SA) := SxA in
-                           bind (fun r => Return _ (r, SA)) (pack nd _ x)
-      | UNPACK => fun SxA => let (x, SA) := SxA in
-                             bind (fun r => Return _ (r, SA)) (unpack nd _ x)
-      | HASH_KEY =>
-        fun SxA =>
-          let (x, SA) := SxA in
-          bind (fun r => Return _ (r, SA))
-               (hash_key nd x)
-      | BLAKE2B =>
-        fun SxA =>
-          let (x, SA) := SxA in
-          bind (fun r => Return _ (r, SA))
-               (blake2b nd x)
-      | SHA256 =>
-        fun SxA =>
-          let (x, SA) := SxA in
-          bind (fun r => Return _ (r, SA))
-               (sha256 nd x)
-      | SHA512 =>
-        fun SxA =>
-          let (x, SA) := SxA in
-          bind (fun r => Return _ (r, SA))
-               (sha512 nd x)
+      | PACK => fun '(x, SA) => bind (fun r => Return _ (r, SA)) (pack nd _ x)
+      | UNPACK => fun '(x, SA) => bind (fun r => Return _ (r, SA)) (unpack nd _ x)
+      | HASH_KEY => fun '(x, SA) => bind (fun r => Return _ (r, SA)) (hash_key nd x)
+      | BLAKE2B => fun '(x, SA) => bind (fun r => Return _ (r, SA)) (blake2b nd x)
+      | SHA256 => fun '(x, SA) => bind (fun r => Return _ (r, SA)) (sha256 nd x)
+      | SHA512 => fun '(x, SA) => bind (fun r => Return _ (r, SA)) (sha512 nd x)
       | CHECK_SIGNATURE =>
-        fun SxyzA =>
-          let (x, SyzA) := SxyzA in
-          let (y, SzA) := SyzA in
-          let (z, SA) := SzA in
-          bind (fun r => Return _ (r, SA))
-               (check_signature nd x y z)
+        fun '(x, (y, (z, SA))) =>
+          bind (fun r => Return _ (r, SA)) (check_signature nd x y z)
       end
     end.
 End semantics.
