src/tez.v
@@ -3,6 +3,7 @@
 Require Import ZArith.
 Require int64.
 Require Eqdep_dec.
+Require error.
 
 Definition mutez : Set := {t : int64.int64 | int64.sign t = false }.
 
@@ -27,13 +28,13 @@ Coercion to_int64 : mutez >-> int64.int64.
 
 Definition to_Z (t : mutez) : Z := int64.to_Z t.
 
-Definition of_int64 (t : int64.int64) : option mutez :=
-  match int64.sign t as b return int64.sign t = b -> option mutez with
-  | false => fun H => Some (exist _ t H)
-  | true => fun _ => None
+Definition of_int64 (t : int64.int64) : error.M mutez :=
+  match int64.sign t as b return int64.sign t = b -> error.M mutez with
+  | false => fun H => error.Return _ (exist _ t H)
+  | true => fun _ => error.Failed _ error.Overflow
   end eq_refl.
 
-Definition of_Z (t : Z) : option mutez :=
+Definition of_Z (t : Z) : error.M mutez :=
   of_int64 (int64.of_Z t).
 
 Definition compare (t1 t2 : mutez) : comparison :=
